Alg/ListProps/Sorted/SetOps.lean
@@ -2,3 +2,406 @@ import Alg.ListProps.Sorted.Merge
 import Alg.ListProps.Sorted.Intersect
 import Alg.ListProps.Sorted.Union
 import Alg.ListProps.Sorted.Difference
+import Alg.Basic
+
+theorem all_eq_to_end :
+  xs.allP (fun i => i = x) ->
+  x::xs = xs ++ [x] := by
+  intro all_eq_first
+  match xs with
+  | [] => rw [List.nil_append]
+  | x'::xs =>
+  rw [all_eq_first.left]
+  congr
+  apply all_eq_to_end all_eq_first.right
+
+#print axioms all_eq_to_end
+
+theorem all_eq_to_sorted [Compare α] {xs: List α} :
+  xs.allP (fun i => i = x) ->
+  xs.sorted := by
+  intro all_eq_first
+  match xs with
+  | [] | [_] => trivial
+  | a::b::xs =>
+  apply And.intro
+  rw [all_eq_first.left, all_eq_first.right.left]
+  apply Compare.le_id
+  apply all_eq_to_sorted all_eq_first.right
+
+#print axioms all_eq_to_sorted
+
+theorem List.sorted.union_def.helper [Compare α]: 
+  ∀{as bs: List α} (x: α) (xs: List α), 
+  xs.allP (fun i => i = x) ->
+  (x::as).sorted ->
+  (x::bs).sorted ->
+  xs ++ (List.sorted_union as bs) = List.sorted_difference (xs ++ List.sorted_merge as bs) (List.sorted_intersect as bs) := by
+  apply sorted.induction
+  {
+    intro bs
+    intro x xs _ _ _
+    rw [
+      sorted_union.empty_left,
+      sorted_merge.empty_left,
+      sorted_intersect.empty_left,
+      sorted_difference.empty_right,
+    ]
+  }
+  {
+    intro a as
+    intro x xs _ _ _
+    rw [
+      sorted_union.empty_right,
+      sorted_merge.empty_right,
+      sorted_intersect.empty_right,
+      sorted_difference.empty_right,
+    ]
+  }
+  {
+    intro a as b bs a_ord_b prev
+    intro x xs xs_eq_x as_sort bs_sort
+    rw [
+      sorted_merge.induct_lt a_ord_b,
+      sorted_intersect.induct_lt a_ord_b,
+      sorted_union.induct_lt a_ord_b,
+    ]
+    have prev_empty := @prev x [] True.intro as_sort.pop_snd bs_sort
+    rw [List.nil_append, List.nil_append] at prev_empty
+    rw [prev_empty]
+    
+    have : ¬containsP (sorted_intersect as (b :: bs)) a := by
+      apply contrapositive (List.sorted_intersect.to_contains _ _ a (as_sort.pop).pop bs_sort.pop)
+      intro con_and_con
+      have ⟨ _, bs_con_a ⟩ := con_and_con
+      have := (bs_sort.pop).not_contains a_ord_b
+      contradiction
+    have : ¬containsP (sorted_intersect as (b :: bs)) x := by
+      apply contrapositive (List.sorted_intersect.to_contains _ _ x (as_sort.pop).pop bs_sort.pop)
+      intro con_and_con
+      have ⟨ _, bs_con_a ⟩ := con_and_con
+      apply (bs_sort.pop).not_contains (Compare.le_lt_trans as_sort.left a_ord_b)
+      assumption
+    have : sorted (a :: sorted_merge as (b :: bs)) := by
+      apply List.sorted_merge.keeps_sorted.helper
+      exact as_sort.pop
+      apply And.intro
+      exact Or.inl a_ord_b
+      exact bs_sort.pop
+      apply List.sorted_merge.keeps_sorted
+      exact (as_sort.pop).pop
+      exact bs_sort.pop
+    have : sorted (sorted_intersect as (b :: bs)) := by
+      apply List.sorted_intersect.keeps_sorted
+      exact (as_sort.pop).pop
+      exact bs_sort.pop
+    
+    rw [List.sorted_difference.all_not_in_right _ _ rfl]
+    rw [List.sorted_difference.not_in_right _ _ rfl]
+    any_goals assumption
+    apply xs_eq_x.map
+    intro y y_eq_x
+    rw [y_eq_x]
+    assumption
+    
+    match xs with
+    | [] =>
+      rw [List.nil_append]
+      assumption
+    | x'::xs =>
+    apply List.sorted.append
+    apply all_eq_to_sorted xs_eq_x
+    assumption
+    have to_end_append : x'::xs = xs ++ [x'] := by
+      apply all_eq_to_end
+      apply xs_eq_x.right.map
+      intro i i_eq_x
+      rw [i_eq_x]
+      exact xs_eq_x.left.symm
+    exact to_end_append
+    rfl
+    rw [xs_eq_x.left]
+    exact as_sort.left
+  }
+  {
+    intro a as b bs a_ord_b prev
+    intro x xs xs_eq_x as_sort bs_sort
+    have a_eq_b := Compare.ord_to_eq a_ord_b
+    rw [sorted_merge.induct_eq a_ord_b] at *
+    have a_ord_x := decEq (Compare.ord a x) .Eq
+    have b_ord_x := decEq (Compare.ord b x) .Eq
+    match dec_and a_ord_x b_ord_x with
+    | .isTrue ⟨ a_ord_x, b_ord_x ⟩  =>
+      rw [Compare.ord_to_eq a_ord_x, Compare.ord_to_eq b_ord_x]
+      rw [sorted_intersect.induct_eq (Compare.ord_id _)] at *
+      rw [List.append_cons, ←all_eq_to_end, List.cons_append]
+      rw [List.append_cons, ←all_eq_to_end, List.cons_append]
+      rw [sorted_difference.induct_eq (Compare.ord_id _)] at *
+      rw [sorted_union.induct_eq (Compare.ord_id _)] at *
+      rw [List.append_cons, ←all_eq_to_end]
+      rw [←List.cons_append]
+      rw [@prev x (x::xs) (⟨ rfl , xs_eq_x ⟩) as_sort.pop_snd bs_sort.pop_snd]
+      assumption
+      assumption
+      assumption
+    | .isFalse not_and_ord => 
+    rw [List.sorted_difference.all_not_in_right _ _ rfl]
+    congr
+    
+    {
+      rw [List.sorted_intersect.induct_eq a_ord_b]
+      rw [List.sorted_union.induct_eq a_ord_b]
+      rw [List.sorted_difference.induct_eq (Compare.ord_id _)]
+      have prev_empty := @prev a [a] (⟨rfl ,True.intro⟩) as_sort.pop (by
+        rw [a_eq_b]
+        exact bs_sort.pop)
+      rw [List.cons_append, List.cons_append, List.nil_append, List.nil_append] at prev_empty
+      rw [←a_eq_b]
+      assumption
+    }
+    
+    {
+      apply xs_eq_x.map
+      intro x' x'_eq_x
+      rw [x'_eq_x]
+      intro con
+      have := List.sorted_intersect.sublist_of_left (a::as) (b::bs)
+      have := (as_sort.pop).contains (this.containsP con)
+      have x_eq_a := Compare.le_to_eq _ _ as_sort.left this
+
+      have := List.sorted_intersect.sublist_of_right (a::as) (b::bs)
+      have := (bs_sort.pop).contains (this.containsP con)
+      have x_eq_b := Compare.le_to_eq _ _ bs_sort.left this
+
+      rw [←x_eq_a, ←x_eq_b] at not_and_ord
+      exact not_and_ord ⟨ Compare.ord_id _, Compare.ord_id _ ⟩
+    }
+    {
+      have : sorted (a :: b :: sorted_merge as bs) := by
+        repeat any_goals apply And.intro
+        exact Or.inr a_ord_b
+        apply List.sorted_merge.keeps_sorted.helper
+        rw [←a_eq_b]
+        exact as_sort.pop
+        exact bs_sort.pop
+        apply List.sorted_merge.keeps_sorted
+        exact (as_sort.pop).pop
+        exact (bs_sort.pop).pop
+      match xs with
+      | [] => rw [List.nil_append]; assumption
+      | x'::xs =>
+        rw [all_eq_to_end]
+        {
+          apply sorted.append
+          rw [←all_eq_to_end]
+          apply all_eq_to_sorted xs_eq_x
+          apply xs_eq_x.right.map
+          intro i i_eq_x
+          apply i_eq_x.trans
+          exact xs_eq_x.left.symm
+          assumption
+          rfl
+          rfl
+          rw [xs_eq_x.left]
+          exact as_sort.left
+        }
+        apply xs_eq_x.right.map
+        intro i i_eq_x
+        apply i_eq_x.trans
+        exact xs_eq_x.left.symm
+    }
+    {
+      apply List.sorted_intersect.keeps_sorted
+      exact as_sort.pop
+      exact bs_sort.pop
+    }
+  }
+  {
+    intro a as b bs a_ord_b prev
+    intro x xs xs_eq_x as_sort bs_sort
+    have b_ord_a := Compare.flip a_ord_b
+    rw [
+      sorted_merge.induct_gt a_ord_b,
+      sorted_intersect.induct_gt a_ord_b,
+      sorted_union.induct_gt a_ord_b,
+    ]
+    have prev_empty := @prev x [] True.intro as_sort bs_sort.pop_snd
+    rw [List.nil_append, List.nil_append] at prev_empty
+    rw [prev_empty]
+    clear prev
+    
+    have : ¬containsP (sorted_intersect (a :: as) bs) b := by
+      apply contrapositive (List.sorted_intersect.to_contains _ _ b as_sort.pop (bs_sort.pop).pop)
+      intro con_and_con
+      have ⟨ as_con_a, _ ⟩ := con_and_con
+      have := (as_sort.pop).not_contains b_ord_a
+      contradiction
+    have : ¬containsP (sorted_intersect (a :: as) bs) x := by
+      apply contrapositive (List.sorted_intersect.to_contains _ _ x as_sort.pop (bs_sort.pop).pop)
+      intro con_and_con
+      have ⟨ as_con_a, _ ⟩ := con_and_con
+      apply (as_sort.pop).not_contains (Compare.le_lt_trans bs_sort.left b_ord_a)
+      assumption
+    have : sorted (b :: sorted_merge (a :: as) bs) := by
+      apply List.sorted_merge.keeps_sorted.helper
+      apply And.intro
+      exact Or.inl b_ord_a
+      exact as_sort.pop
+      exact bs_sort.pop
+      apply List.sorted_merge.keeps_sorted
+      exact as_sort.pop
+      exact (bs_sort.pop).pop
+    have : sorted (sorted_intersect (a :: as) bs) := by
+      apply List.sorted_intersect.keeps_sorted
+      exact as_sort.pop
+      exact (bs_sort.pop).pop
+
+    rw [List.sorted_difference.all_not_in_right _ _ rfl]
+    rw [List.sorted_difference.not_in_right _ _ rfl]
+    any_goals assumption
+    apply xs_eq_x.map
+    intro y y_eq_x
+    rw [y_eq_x]
+    assumption
+    
+    match xs with
+    | [] =>
+      rw [List.nil_append]
+      assumption
+    | x'::xs =>
+    apply List.sorted.append
+    apply all_eq_to_sorted xs_eq_x
+    assumption
+    have to_end_append : x'::xs = xs ++ [x'] := by
+      apply all_eq_to_end
+      apply xs_eq_x.right.map
+      intro i i_eq_x
+      rw [i_eq_x]
+      exact xs_eq_x.left.symm
+    exact to_end_append
+    rfl
+    rw [xs_eq_x.left]
+    exact bs_sort.left
+  }
+
+#print axioms List.sorted.union_def.helper
+
+theorem List.sorted.union_def [Compare α]: 
+  ∀{as bs: List α }, 
+  as.sorted ->
+  bs.sorted ->
+  as.sorted_union bs =
+  (as.sorted_merge bs).sorted_difference (as.sorted_intersect bs) := by
+  apply List.sorted.induction
+  {
+    intro bs
+    intro _ _
+    rw [
+      sorted_union.empty_left,
+      sorted_merge.empty_left,
+      sorted_intersect.empty_left,
+      sorted_difference.empty_right,
+    ]
+  }
+  {
+    intro a as
+    intro _ _
+    rw [
+      sorted_union.empty_right,
+      sorted_merge.empty_right,
+      sorted_intersect.empty_right,
+      sorted_difference.empty_right,
+    ]
+  }
+  {
+    intro a as b bs a_ord_b prev
+    intro as_sort bs_sort
+    rw [
+      sorted_union.induct_lt a_ord_b,
+      sorted_merge.induct_lt a_ord_b,
+      sorted_intersect.induct_lt a_ord_b,
+    ]
+    rw [List.sorted_difference.not_in_right _ _ rfl]
+    congr
+    apply prev
+    exact as_sort.pop
+    exact bs_sort
+    {
+      intro con
+      have := List.sorted_intersect.sublist_of_right as (b::bs)
+      have := this.containsP con
+      have := bs_sort.not_contains a_ord_b
+      contradiction
+    }
+    {
+      apply List.sorted_merge.keeps_sorted.helper
+      assumption
+      apply And.intro
+      exact Or.inl a_ord_b
+      assumption
+      apply List.sorted_merge.keeps_sorted
+      exact as_sort.pop
+      assumption
+    }
+    {
+      apply List.sorted_intersect.keeps_sorted
+      exact as_sort.pop
+      exact bs_sort
+    }
+  }
+  {
+    intro a as b bs a_ord_b _
+    intro as_sort bs_sort
+    have a_eq_b := Compare.ord_to_eq a_ord_b
+    rw [
+      sorted_union.induct_eq a_ord_b,
+      sorted_merge.induct_eq a_ord_b,
+      sorted_intersect.induct_eq a_ord_b,
+      sorted_difference.induct_eq (Compare.ord_id _),
+    ]
+
+    have := List.sorted.union_def.helper a [b] (⟨ a_eq_b.symm, True.intro ⟩) as_sort (by
+      rw [a_eq_b]
+      exact bs_sort)
+    rw [List.cons_append, List.cons_append, List.nil_append, List.nil_append] at this
+    rw [←this]
+    congr
+  }
+  {
+    intro a as b bs a_ord_b prev
+    intro as_sort bs_sort
+    rw [
+      sorted_union.induct_gt a_ord_b,
+      sorted_merge.induct_gt a_ord_b,
+      sorted_intersect.induct_gt a_ord_b,
+    ]
+    rw [List.sorted_difference.not_in_right _ _ rfl]
+    congr
+    apply prev
+    exact as_sort
+    exact bs_sort.pop
+    {
+      intro con
+      have := List.sorted_intersect.sublist_of_left (a::as) bs
+      have := this.containsP con
+      have := as_sort.not_contains (Compare.flip a_ord_b)
+      contradiction
+    }
+    {
+      apply List.sorted_merge.keeps_sorted.helper
+      apply And.intro
+      exact Or.inl (Compare.flip a_ord_b)
+      assumption
+      assumption
+      apply List.sorted_merge.keeps_sorted
+      assumption
+      exact bs_sort.pop
+    }
+    {
+      apply List.sorted_intersect.keeps_sorted
+      exact as_sort
+      exact bs_sort.pop
+    }
+  }
+
+#print axioms List.sorted.union_def
